Stlc.v
@@ -1,4 +1,91 @@
 Add LoadPath "/Users/chenshen/src/sf/".
+
+
 Require Import Maps.
 Require Import Smallstep.
 Require Import Types.
+
+
+
+Module STLC.
+
+Inductive ty : Type :=
+  | TBool : ty
+  | TArrow : ty -> ty -> ty.
+
+Inductive tm : Type :=
+  | tvar : id -> tm
+  | tapp : tm -> tm -> tm
+  | tabs : id -> ty -> tm -> tm
+  | ttrue : tm
+  | tfalse : tm
+  | tif : tm -> tm -> tm -> tm.
+
+
+Definition x := (Id 0).
+Definition y := (Id 1).
+Definition z := (Id 2).
+Hint Unfold x.
+Hint Unfold y.
+Hint Unfold z.
+
+(** [idB = \x:Bool. x] *)
+
+Notation idB :=
+  (tabs x TBool (tvar x)).
+
+(** [idBB = \x:Bool->Bool. x] *)
+
+Notation idBB :=
+  (tabs x (TArrow TBool TBool) (tvar x)).
+
+(** [idBBBB = \x:(Bool->Bool) -> (Bool->Bool). x] *)
+
+Notation idBBBB :=
+  (tabs x (TArrow (TArrow TBool TBool)
+                      (TArrow TBool TBool))
+    (tvar x)).
+
+(** [k = \x:Bool. \y:Bool. x] *)
+
+Notation k := (tabs x TBool (tabs y TBool (tvar x))).
+
+(** [notB = \x:Bool. if x then false else true] *)
+
+Notation notB := (tabs x TBool (tif (tvar x) tfalse ttrue)).
+
+Inductive value : tm -> Prop :=
+  | v_abs : forall x T t,
+      value (tabs x T t)
+  | v_true :
+      value ttrue
+  | v_false :
+      value tfalse.
+
+Hint Constructors value.
+
+Fixpoint test1 (n :nat) : nat :=
+  match n with 
+  | O => if Nat.eqb n n then 1 else 2
+  | _ => n
+  end.
+
+Reserved Notation "'[' x ':=' s ']' t" (at level 20).
+
+Fixpoint subst (x:id) (s:tm) (t:tm) : tm :=
+  match t with
+  | tvar x' =>
+      if beq_id x x' then s else t
+  | tabs x' T t1 =>
+      tabs x' T (if beq_id x x' then t1 else ([x:=s] t1))
+  | tapp t1 t2 =>
+      tapp ([x:=s] t1) ([x:=s] t2)
+  | ttrue =>
+      ttrue
+  | tfalse =>
+      tfalse
+  | tif t1 t2 t3 =>
+      tif ([x:=s] t1) ([x:=s] t2) ([x:=s] t3)
+  end
+
+where "'[' x ':=' s ']' t" := (subst x s t).
